% This is Plain TeX file dcon_gen.tex.

\magnification=\magstep2

\font\bfbig=cmbx12
\font\ssbf=cmssbx10
\def\t#1{\hbox{\ssbf #1}}
\def\v#1{\hbox{\bf #1}}

\centerline{\bfbig Straight Fieldline Coordinate System}
\medskip

$$ {\cal J} \equiv (\nabla \psi \cdot \nabla \theta 
	\times \nabla \zeta)^{-1}, \quad
{\cal F}'(\psi, \theta, \zeta) 
	\equiv {\partial {\cal F} \over \partial \psi}
\eqno(1) $$

$$ {\cal F}(\psi,\theta,\zeta) 
= {\cal F}(\psi,\theta + 1,\zeta)
= {\cal F}(\psi,\theta,\zeta + 1) 
\eqno(2) $$

$$ |\nabla \phi|^2 = {1 \over R^2}, \quad
\nabla \phi \cdot \nabla \psi = \nabla \theta \cdot \nabla \phi = 0
\eqno(3) $$

$$ \phi(\psi,\theta,\zeta) 
	= 2 \pi \zeta + \nu(\psi,\theta), \quad
\nu(\psi,\theta) = \nu(\psi,\theta+1)
\eqno(4) $$

\bigskip
\centerline{\bfbig Axisymmetric Equilibrium Magnetic Field}
\medskip

$$ \v{B} \equiv f \nabla \phi
	+ {\chi' \over 2 \pi} \nabla \phi \times \nabla \psi
= \chi' \left[ \nabla \zeta
	- q(\psi) \nabla \theta \right] \times \nabla \psi
\eqno(5) $$ 

$$ 
B_\psi \equiv \v{B} \cdot \nabla \psi = 0, \quad
B_\theta \equiv \v{B} \cdot \nabla \theta = {\chi'\over {\cal J}}, \quad
B_\zeta \equiv \v{B} \cdot \nabla \zeta = q {\chi' \over {\cal J}}
\eqno(6) $$

$$ q(\psi) \equiv {\v{B} \cdot \nabla \zeta \over \v{B} \cdot \nabla \theta}
= {f \over 2 \pi \chi'} \int_0^1 d\theta \ {{\cal J} \over R^2}, \quad
\nu(\psi,\theta) = {f \over 2 \pi \chi'} \int d\theta 
	{{\cal J} \over R^2} - 2 \pi q \theta
\eqno(7) $$

$$ \v{B} \cdot \nabla {\cal F} = \v{B} \cdot \nabla \theta
	\left( {\partial \over \partial \theta} 
	+ q {\partial \over \partial \zeta} \right) 
{\cal F}(\psi,\theta,\zeta) \eqno(8) $$

\bigskip
\centerline{\bfbig Equilibrium Current and Pressure}
\medskip

$$ \v{J} = \nabla \times \v{B} \eqno(9) $$

$$ \eqalign{
J_\psi = {2 \pi \over {\cal J}} 
	{\partial f \over \partial \theta} = 0, \quad 
J_\theta = - {2 \pi \over {\cal J}} {\partial f \over \partial \psi}, \quad 
J_\phi = {1 \over 2 \pi} \nabla \cdot 
	\left( {1 \over R^2} \nabla \chi \right)
} \eqno(10) $$

$$ \v{J} \times \v{B} = \nabla P, \quad
J_\zeta = q J_\theta - {P' \over \chi'}
	= -{2\pi q f' \over {\cal J}} - {P' \over \chi'}
\eqno(11) $$

$$ \Delta^* \chi 
	\equiv R^2 \nabla \cdot \left( {1 \over R^2} \nabla \chi \right)
	= - {4 \pi^2 \over \chi'} (ff' + R^2 P')
\eqno(12) $$

\vfill\eject
\centerline {\bfbig  Velocity and Vector Potential}

$$ \v{v} = {\cal J} \left( \dot{\psi} \nabla \theta \times \nabla \zeta
	+ \dot{\theta} \nabla \zeta \times \nabla \psi
	+ \dot{\zeta} \nabla \psi \times \nabla \theta \right)
\eqno(13) $$

$$ \v{A} = \Phi \nabla \theta - \chi \nabla \zeta , \quad
\Phi' = q \chi'
\eqno(14) $$

\bigskip
\centerline {\bfbig  Metric Tensor}

$$ \eqalign{
g_{11} &= |\nabla \theta \times \nabla \zeta|^2 \hskip0.25in
g_{23} = g_{32} = (\nabla \zeta \times \nabla \psi)
	\cdot (\nabla \psi \times \nabla \theta) \cr
g_{22} &= |\nabla \zeta \times \nabla \psi|^2 \hskip0.25in
g_{31} = g_{13} = (\nabla \psi \times \nabla \theta)
	\cdot (\nabla \theta \times \nabla \zeta) \cr
g_{33} &= |\nabla \psi \times \nabla \theta|^2 \hskip0.25in
g_{12} = g_{21} = (\nabla \theta \times \nabla \zeta)
	\cdot (\nabla \zeta \times \nabla \psi)
} \eqno(15) $$

$$ g_{ij} g^{jk} = \delta_i^k \eqno(16) $$

\bigskip
\centerline {\bfbig  Lagrangian}

$$ \eqalign{ L 
=& {1 \over 2} m v^2 + e (\v{A} \cdot \v{v} - \varphi) \cr
=& {m {\cal J}^2 \over 2} \left(
	g_{11} \dot{\psi}^2 + g_{22} \dot{\theta}^2 + g_{33} \dot{\zeta}^2
	+ 2 g_{12} \dot{\psi} \dot{\theta} 
	+ 2 g_{23} \dot{\theta} \dot{\zeta}
	+ 2 g_{31} \dot{\zeta} \dot{\psi} \right) \cr
&+ e \left(\Phi \dot{\theta} - \chi \dot{\zeta} - \varphi \right)
} \eqno(17) $$

\bigskip
\centerline {\bfbig  Canonical Momenta}

$$ \eqalign{
p_\psi \equiv& {\partial L \over \partial \dot{\psi}}
	= m {\cal J}^2 \left( g_{11} \dot{\psi} + g_{12} \dot{\theta} 
	+ g_{13} \dot{\zeta} \right) \cr
p_\theta \equiv& {\partial L \over \partial \dot{\theta}}
	= m {\cal J}^2 \left( g_{21} \dot{\psi} + g_{22} \dot{\theta} 
	+ g_{23} \dot{\zeta} \right) 
	+ e \Phi \cr
p_\zeta \equiv& {\partial L \over \partial \dot{\zeta}}
	= m {\cal J}^2 \left( g_{31} \dot{\psi} + g_{32} \dot{\theta} 
	+ g_{33} \dot{\zeta} \right)
	- e \chi \cr
} \eqno(18) $$

\vfill\eject
\centerline {\bfbig Hamiltonian}

$$ \eqalign{ H 
\equiv& \dot{\psi} p_\psi + \dot{\theta} p_\theta + \dot{\zeta} p_\zeta - L \cr
=& {m {\cal J}^2 \over 2} \left(
	g_{11} \dot{\psi}^2 + g_{22} \dot{\theta}^2 + g_{33} \dot{\zeta}^2
	+ 2 g_{12} \dot{\psi} \dot{\theta} 
	+ 2 g_{23} \dot{\theta} \dot{\zeta}
	+ 2 g_{31} \dot{\zeta} \dot{\psi} \right)
	+ e \varphi \cr
=& {1 \over 2m {\cal J}^2} \left\{
	g^{11} p_\psi^2 + g^{22} (p_\theta + e\Phi)^2 
	+ g^{33} (p_\zeta - e\chi)^2 \right. \cr
&\quad 
	+ 2 p_\psi \left[ g^{12} (p_\theta - e\Phi)
	+ g^{31} (p_\zeta + e\chi) \right] \cr
&\quad \left. 
	+ 2 g^{23} (p_\theta - e\Phi) (p_\zeta + e\chi) \right\}
	 + e \varphi \cr
} \eqno(19) $$

\bigskip
\centerline {\bfbig Hamilton's Equations}

$$ \eqalign{ 
\dot{\psi} =& { \partial H \over \partial p_\psi }
	= {1 \over m {\cal J}^2} \left[ g^{11} p_\psi 
	+ g^{12} \left( p_\theta - e \Phi \right)
	+ g^{13} \left( p_\zeta + e \chi \right)
	\right] \cr
\dot{\theta} =& { \partial H \over \partial p_\theta }
	= {1 \over m {\cal J}^2} \left[ g^{21} p_\psi 
	+ g^{22} \left( p_\theta - e \Phi \right)
	+ g^{23} \left( p_\zeta + e \chi \right)
	\right] \cr
\dot{\zeta} =& { \partial H \over \partial p_\zeta }
	= {1 \over m {\cal J}^2} \left[ g^{31} p_\psi 
	+ g^{32} \left( p_\theta - e \Phi \right)
	+ g^{33} \left( p_\zeta + e \chi \right)
	\right]
} \eqno(20) $$

$$ 
\dot{p}_\psi = - {\partial H \over \partial \psi}, \quad
\dot{p}_\theta = - {\partial H \over \partial \theta}, \quad
\dot{p}_\zeta = - {\partial H \over \partial \zeta}
\eqno(21) $$

\vfill\eject
\centerline {\bfbig Matrix Formulation}

$$ 
\v{x} \equiv \left( \matrix{\psi \cr \theta \cr \zeta} \right), \quad
\dot{\v{x}} \equiv \left( \matrix{\dot{\psi} 
	\cr \dot{\theta} \cr \dot{\zeta}} \right), \quad
\v{v} \equiv \left( \matrix{\dot{R} 
	\cr \dot{Z} \cr R \dot{\phi}} \right)
\eqno(22) $$

$$
\v{p} \equiv \left( \matrix{p_\psi \cr p_\theta \cr p_\zeta} \right), \quad
\v{A} \equiv \left( \matrix{0 \cr \Phi \cr - \chi} \right)
\eqno(23) $$

$$ \t{J} \equiv \left( \matrix{
	\partial R / \partial \psi 
	&\partial R / \partial \theta
	&0 \cr
	\partial Z / \partial \psi 
	&\partial Z / \partial \theta
	&0 \cr
	R \partial \phi / \partial \psi 
	&R \partial \phi / \partial \theta
	&2 \pi R} \right), \quad
\t{g} = \t{g}^T = {\t{J}^T \t{J} \over {\cal J}^2}, \quad
\t{G} \equiv \t{g}^{-1}
\eqno(24) $$
	
$$ \v{v} = \t{J} \dot{\v{x}}, \quad
\v{p} - e \v{A} = m {\cal J}^2 \t{g} \dot{\v{x}} 
	= m \t{J}^T \t{J} \dot{\v{x}} 
	= m \v{J}^T \v{v}
\eqno(25) $$

$$ \eqalign{H 
=& {m v^2 \over 2} \cr
=& {1 \over 2 m {\cal J}^2} (\v{p} - e \v{A})^T \t{G} (\v{p} - e \v{A}) \cr
=& {1 \over 2 m} (\v{p} - e \v{A})^T \t{J}^{-1} 
	\t{J}^{-1T} (\v{p} - e \v{A}) \cr
} \eqno(26) $$

$$ \dot{\v{x}} = {\partial H \over \partial \v{p}} 
	= {1 \over m {\cal J}^2} \t{G} (\v{p} - e \v{A})
	= {1 \over m} \t{J}^{-1} \t{J}^{-1T} (\v{p} - e \v{A})
	= \t{J}^{-1} \v{v}
\eqno(27) $$

$$ \dot{\v{p}} = - {\partial H \over \partial \v{x}} 
\eqno(28) $$

\end
