% This is Plain TeX file dcon_gen.tex.

\magnification=\magstep2

\font\bfbig=cmbx12
\font\ssbf=cmssbx10
\def\t#1{\hbox{\ssbf #1}}
\def\v#1{\hbox{\bf #1}}
\def\b{\hat{\bf b}}

\centerline{\bfbig Ballooning Representation}
\medskip

$$ \varphi(\psi,\theta,\beta) 
	= \varphi(\psi,\theta,\beta+1) 
	= \varphi(\psi,\theta+1,\beta-q) 
\eqno(1) $$

$$ \varphi(\psi,\theta,\beta)  = \sum_{l=-\infty}^\infty 
	\hat{\varphi} (\psi,\theta-l)
	\exp \left[ - 2 \pi i n 
	\left( \beta + l q \right) \right] 
\eqno(2) $$

$$ \eqalign{
\beta \equiv& \zeta - q \theta + \int q' \theta_0(\psi) d\psi \cr
\nabla \beta =& \nabla \zeta - q \nabla \theta 
	- q' (\theta - \theta_0) \nabla \psi \cr
|\nabla \beta|^2 
=& |\nabla \zeta - q \nabla \theta|^2 
	+ q'^2 (\theta - \theta_0)^2 |\nabla \psi|^2 \cr
&- 2 q' (\theta - \theta_0) 
	(\nabla \zeta - q \nabla \theta ) \cdot \nabla \psi \cr
} \eqno(3) $$

\bigskip
\centerline{\bfbig Ideal Marginal Ballooning Equation}
\medskip

$$ \v{B} \cdot \nabla \left( {|\nabla \beta|^2 \over B^2}
	\v{B} \cdot \nabla \hat{\varphi} \right) 
	+ 2 {P' \over \chi'} \kappa_w \hat{\varphi} = 0
\eqno(4) $$

$$ {\chi' \over {\cal J}} {\partial \over \partial \theta} 
	\left( {|\nabla \beta|^2 \over B^2}
	{\chi' \over {\cal J}} 
	{\partial \hat{\varphi} \over \partial \theta} \right) 
	+ 2 {P' \over \chi'} \kappa_w \hat{\varphi} = 0
\eqno(5) $$

$$ 
{\partial \v{u} \over \partial \theta} = \t{L} \v{u}, \quad
\v{u} \equiv \left( \matrix{ \hat{\varphi} \cr
	{|\nabla \beta|^2 \over B^2} {\chi' \over {\cal J}} 
	{\partial\hat{\varphi}  \over \partial \theta} 
	} \right), \quad
\t{L} \equiv {{\cal J} \over \chi'} \left( \matrix{ 0 
	& {B^2 \over |\nabla \beta|^2} \cr
	- 2 {P' \over \chi'} \kappa_w & 0 } \right)
\eqno(6) $$

\vfill\eject
\centerline {\bfbig Curvature}
\medskip

$$ \kappa \equiv \b \cdot \nabla \b
	= (\nabla \times \b) \times \b, \quad
\b \equiv {\v{B} \over B}
\eqno(7) $$

$$ \eqalign{ \nabla P 
=& \v{J} \times \v{B} = (\nabla \times \v{B}) \times \v{B} 
	= \left[ \nabla \times (B \b) \right] \times \v{B} \cr
=& \left( B \nabla \times \b + \nabla B \times \b \right) \times \v{B}
	= B^2 \kappa - B \left( \t{I} - \b\b \right) \cdot \nabla B
} \eqno(8) $$

$$ B^2 \kappa = \nabla P + B \left( \t{I} - \b\b \right) \cdot \nabla B
\eqno(9) $$

$$ \eqalign{\kappa_s 
\equiv& {\kappa \times \v{B} \over B^2} \cdot \nabla \psi 
	= (\nabla \times \b) \times \b
	\cdot {\v{B} \times \nabla \psi \over B^2}
	= - {1 \over B} \nabla \cdot \left( 
	{\v{B} \times \nabla \psi \over B} \right) \cr
=& - {1 \over {\cal J} B} {\partial \over \partial \theta} \left( 
	{\cal J} {\v{B} \cdot \nabla \psi \times \nabla \theta \over B} 
	\right)
	= - {\pi f \over {\cal J}} {\partial \over \partial \theta} 
	\left( {1 \over B^2} \right)
} \eqno(10) $$

$$ \eqalign{ \kappa_w 
\equiv& {\kappa \times \v{B} \over B^2} \cdot \nabla \beta \cr
=& (\nabla \times \b) \times \b
	\cdot {\v{B} \times \nabla \beta \over B^2}
	= - {1 \over B} \nabla \cdot \left( 
	{\v{B} \times \nabla \beta \over B} \right) \cr
=& - {1 \over {\cal J} B} {\partial \over \partial \psi} \left( 
	{\cal J} {\v{B} \cdot \nabla \beta \times \nabla \psi \over B} 
	\right)
	- {1 \over {\cal J} B} {\partial \over \partial \theta} \left( 
	{\cal J} {\v{B} \cdot \nabla \beta \times \nabla \theta \over B} 
	\right) \cr
=& - {1 \over {\cal J} B} {\partial \over \partial \psi} \left( 
	{{\cal J} B \over \chi'} \right)
	+ {1 \over {\cal J} B} {\partial \over \partial \theta} \left(
	{\cal J} {\v{B} \cdot \nabla \theta \times \nabla \zeta \over B}  
	\right) + {2 \pi f q' \over B^2 {\cal J}} - q' \theta \kappa_s \cr
=& \left[ \nabla P + B \left( \t{I} - \b\b \right) \cdot \nabla B \right] 
	\cdot {\v{B} \times \nabla \beta \over B^4} \cr
=& {1 \over \chi'} \left( {P' \over B^2} 
	+ {1 \over B} {\partial B \over \partial \psi} \right)
	- \left( {\v{B} \cdot \nabla \theta \times \nabla \zeta \over
	B^3}  \right) {\partial B \over \partial \theta} - q' \theta \kappa_s
} \eqno(11) $$

$$ \eqalign{ 2 \kappa_w 
=& {1 \over \chi'} \left( 
	{P' \over B^2} + {\chi'' \over \chi'} 
	- {{\cal J}' \over {\cal J}} \right)
	+ {2\pi f q' \over B^2 {\cal J}}
+ {1 \over {\cal J}} {\partial \over \partial \theta} \left(
	{\cal J} {\v{B} \cdot \nabla \theta \times \nabla \zeta \over B^2}  
	\right)  - 2 q' \theta \kappa_s
} \eqno(12) $$

\vfill\eject
\centerline{\bfbig Large $\theta$ Limit}
\medskip

$$ 
{\partial \v{u} \over \partial \theta} = \t{L} \v{u}, \quad
\t{L} \equiv {{\cal J} \over \chi'} \left( \matrix{ 0 
	& B^2 / |\nabla \beta|^2 \cr
	- 2 P' \kappa_w / \chi' & 0 } \right)
\eqno(13) $$

$$ \nabla \beta = |\nabla \zeta - q \nabla \theta|^2 
	- 2 q' \theta (\nabla \zeta - q \nabla \theta ) 
	\cdot \nabla \psi
	+ q'^2 \theta^2 |\nabla \psi|^2 
\eqno(14) $$

$$ \kappa_w =\kappa_n - q' \theta \kappa_s, \quad
\kappa_s = - {1 \over {\cal J}} {\partial \over \partial \theta} 
	\left( {\pi f \over B^2} \right)
\eqno(15) $$


$$ \v{u} = \t{R} \v{v}, \quad
\t{R} = \left( \matrix{ \theta^{-1/2} & 0 \cr 0 & \theta^{1/2} }
	\right), \quad  
{\partial \v{v} \over \partial \theta} = \t{M} \v{v}
\eqno(16) $$

$$ \eqalign{ \t{M} 
=& \t{R}^{-1} \left( \t{L} \t{R} - \t{R}' \right) \cr
=& {{\cal J} \over \chi'} \left( \matrix{ 1/2 \theta
	& B^2 \theta / |\nabla \beta|^2 \cr
	- 2 P' \kappa_w / \chi' \theta & -1/2 \theta } \right) \cr
=& \t{M}_{-1} + \theta^{-1} \sum_{k=0}^{\infty} 
	\theta^{-k} \t{M}_k (\theta), \quad
\t{M}_k(\theta+1) = \t{M}_k(\theta)
} \eqno(17) $$

$$ \t{v} = \theta^\alpha \sum_{k=0}^{\infty} \theta^{-k} 
	\v{v}^{(k)} (\theta),  \quad
\v{v}^{(k)}(\theta+1) = \v{v}^{(k)}(\theta)
\eqno(18) $$

\bigskip
\centerline {\bfbig Lowest Order}
\medskip

$$ \t{M}_{-1}
= \left( \matrix{ 0 & 0 \cr 
	2 {\cal J} P' q' \kappa_s / \chi'^2 
	& 0 } \right)
= - {\partial \over \partial \theta}
\left( \matrix{ 0 & 0 \cr 2 \pi f P' q' / \chi'^2 B^2 & 0 } \right)
\eqno(19) $$

$$ \t{S} \equiv \left( \matrix{ 1 & 0 \cr 
	- 2 \pi f P' q' / \chi'^2 B^2
	& 1 } \right), \quad
\t{S}^T \t{J} \t{S} = \t{J}
\eqno(20) $$

$$ \t{N}_{-1} \equiv \t{S}^{-1} \left( \t{M}_k \t{S} 
	- {\partial \t{S} \over \partial \theta} \right) = 0
\eqno(21) $$

$$ {\partial \t{v}^{(0)} \over \partial \theta} - \t{M}_{-1} \v{v}^{(0)}
	= 0, \quad
\v{v}^{(0)} = \t{S} \v{w}^{(0)}, \quad
{\partial \t{w}^{(0)} \over \partial \theta} = 0
\eqno(22) $$

\vfill\eject
\centerline{\bfbig Higher Order, General Considerations}
\medskip

$$ {\partial \v{v}^{(k+1)} \over \partial \theta} 
	- \t{M}_{-1} \v{v}^{(k+1)}
	= \left[ \t{M}_0 -  \left( \alpha + k \right) 
	\t{I} \right] \v{v}^{(k)}
	+ \sum_{l=1}^k \t{M}_l \v{v}^{(k-l)}
\eqno(23) $$

$$ \v{v}^{(k)} = \t{S} \v{w}^{(k)}, \quad
\t{N}_k \equiv \t{S}^{-1} \t{M}_k \t{S}, \quad k \ge 0
\eqno(24) $$

$$ {\partial \v{w}^{(k+1)} \over \partial \theta} 
	= \left[ \t{N}_0 -  \left( \alpha + k \right) 
	\t{I} \right] \v{w}^{(k)}
	+ \sum_{l=1}^k \t{N}_l \v{w}^{(k-l)}
\eqno(25) $$

$$ \left< {\cal F} \right> \equiv \int_0^1 {\cal F} d\theta
\eqno(26) $$

$$ \left< \left[ \t{N}_0 -  \left( \alpha + k \right) 
	\t{I} \right] \v{w}^{(k)}
	+ \sum_{l=1}^k \t{N}_l \v{w}^{(k-l)} \right> = 0
\eqno(27) $$

\bigskip
\centerline{\bfbig First Order}
\medskip

$$ \t{M}_0 = {{\cal J} \over \chi'} \left( \matrix{ 
	1/2 & B^2 / q'^2 |\nabla \psi|^2 \cr
	- 2 P' \kappa_n / \chi' & -1/2 } \right), \quad
\t{N}_0 \equiv \t{S}^{-1} \t{M}_0 \t{S}
\eqno(28) $$

$$ \left[ \left<\t{N}_0\right> - \alpha \t{I} \right] \v{w}^{(0)} = 0,
	\quad 
\det \left[ \left<\t{N}_0\right> - \alpha \t{I} \right] = 0, \quad
\alpha = \pm \left( - D_I \right)^{1/2}
\eqno(29) $$

$$ {\partial \v{w}^{(1)} \over \partial \theta} 
	= \left( \t{N}_0 - \alpha \t{I} \right) \v{w}^{(0)}
\eqno(30) $$

\end
