% This is Plain TeX file dcon_gen.tex.

\magnification=\magstep2

\font\bfbig=cmbx12
\font\ssbf=cmssbx10
\def\t#1{\hbox{\ssbf #1}}
\def\v#1{\hbox{\bf #1}}

\centerline{\bfbig Straight Fieldline Coordinate System}
\medskip

$$ {\cal J} \equiv (\nabla \psi \cdot \nabla \theta 
	\times \nabla \zeta)^{-1}, \quad
{\cal F}'(\psi, \theta, \zeta) 
	\equiv {\partial {\cal F} \over \partial \psi}
\eqno(1) $$

$$ {\cal F}(\psi,\theta,\zeta) 
= {\cal F}(\psi,\theta + 1,\zeta) 
= {\cal F}(\psi,\theta,\zeta + 1) 
\eqno(2) $$

$$ |\nabla \phi|^2 = {1 \over R^2}, \quad
\nabla \phi \cdot \nabla \psi = \nabla \theta \cdot \nabla \phi = 0
\eqno(3) $$

$$ \phi(\psi,\theta,\zeta) 
	= 2 \pi \zeta + \nu(\psi,\theta), \quad
\nu(\psi,\theta) = \nu(\psi,\theta+1)
\eqno(4) $$

\bigskip
\centerline{\bfbig Axisymmetric Equilibrium Magnetic Field}
\medskip

$$ \v{B} \equiv f \nabla \phi
	+ {\chi' \over 2 \pi} \nabla \phi \times \nabla \psi
= \chi' \left[ \nabla \zeta
	- q(\psi) \nabla \theta \right] \times \nabla \psi
\eqno(5) $$ 

$$ 
B_\psi \equiv \v{B} \cdot \nabla \psi = 0, \quad
B_\theta \equiv \v{B} \cdot \nabla \theta = {\chi'\over {\cal J}}, \quad
B_\zeta \equiv \v{B} \cdot \nabla \zeta = q {\chi' \over {\cal J}}
\eqno(6) $$

$$ q(\psi) \equiv {\v{B} \cdot \nabla \zeta \over \v{B} \cdot \nabla \theta}
= {f \over 2 \pi \chi'} \int_0^1 d\theta \ {{\cal J} \over R^2}, \quad
\nu(\psi,\theta) = {f \over 2 \pi \chi'} \int d\theta 
	{{\cal J} \over R^2} - 2 \pi q \theta
\eqno(7) $$

$$ \v{B} \cdot \nabla {\cal F} = \v{B} \cdot \nabla \theta
	\left( {\partial \over \partial \theta} 
	+ q {\partial \over \partial \zeta} \right) 
{\cal F}(\psi,\theta,\zeta) \eqno(8) $$

\bigskip
\centerline{\bfbig Equilibrium Current and Pressure}
\medskip

$$ \v{J} = \nabla \times \v{B} \eqno(9) $$

$$ \eqalign{
J_\psi = {2 \pi \over {\cal J}} 
	{\partial f \over \partial \theta} = 0, \quad 
J_\theta = - {2 \pi \over {\cal J}} {\partial f \over \partial \psi}, \quad 
J_\phi = {1 \over 2 \pi} \nabla \cdot 
	\left( {1 \over R^2} \nabla \chi \right)
} \eqno(10) $$

$$ \v{J} \times \v{B} = \nabla P, \quad
J_\zeta = q J_\theta - {P' \over \chi'}
	= -{2\pi q f' \over {\cal J}} - {P' \over \chi'}
\eqno(11) $$

$$ \Delta^* \chi 
	\equiv R^2 \nabla \cdot \left( {1 \over R^2} \nabla \chi \right)
	= - {4 \pi^2 \over \chi'} (ff' + R^2 P')
\eqno(12) $$

\vfill\eject
\centerline{\bfbig Perturbed Displacement and Magnetic Field}
\medskip

$$ \xi = {\cal J} \left( 
	\xi_\psi \nabla \theta \times \nabla \zeta
	+ \xi_\theta \nabla \zeta \times \nabla \psi
	+ \xi_\zeta \nabla \psi \times \nabla \theta \right)
\eqno(13) $$

$$ \xi_s 
\equiv {\cal J} \left( \xi \times \v{B} \right) 
	\cdot \left( \nabla \theta \times \nabla \zeta \right)
= \chi' (q \xi_\theta - \xi_\zeta)
\eqno(14) $$

$$ \eqalign{ \v{Q} 
=& \nabla \times (\xi \times \v{B}) \cr
=& {\cal J} \left( Q_\psi \nabla \theta \times \nabla \zeta
+ Q_\theta \nabla \zeta \times \nabla \psi
+ Q_\zeta \nabla \psi \times \nabla \theta \right)
} \eqno(15) $$

$$ \eqalign{
Q_\psi &= {\chi' \over {\cal J}} \left( 
	{\partial \over \partial \theta}
	+ q {\partial \over \partial \zeta} \right) 
	\xi_\psi \cr
Q_\theta &= - {1 \over {\cal J}}
	{\partial \over \partial \psi}
	\left( \chi' \xi_\psi \right)
	+ {1 \over {\cal J}} 
	{\partial \xi_s \over \partial \zeta} \cr
Q_\zeta &= - {1 \over {\cal J}}
	{\partial \over \partial \psi}
	\left( q \chi' \xi_\psi \right)
	- {1 \over {\cal J}} 
	{\partial \xi_s \over \partial \theta} 
} \eqno(16) $$

$$ \eqalign{\v{Q} 
=& \nabla \xi_s \times  \nabla \psi
	+ (\nabla \theta \times \nabla \zeta) 
	{\cal J} \v{B} \cdot \nabla \xi_\psi - \v{B} \xi'_\psi \cr
&- \left[ \chi'' \nabla \zeta \times \nabla \psi
	+ (q \chi')' \nabla \psi \times \nabla \theta \right] \xi_\psi
} \eqno(17) $$

\bigskip
\centerline{\bfbig Fourier Representation}
\medskip

$$ \eqalign{
\xi_s(\psi,\theta,\zeta) 
	&= \sum_{m=-\infty}^\infty \sum_{n=-\infty}^\infty
	u_{m,n}(\psi) e^{i(m\theta-n\zeta)} \cr
\xi_\psi(\psi,\theta,\zeta) 
	&= \sum_{m=-\infty}^\infty \sum_{n=-\infty}^\infty
	v_{m,n}(\psi) e^{i(m\theta-n\zeta)}
} \eqno(18) $$

$$ \eqalign{
\xi_s(\psi,\theta,\zeta) &= \xi_s^*(\psi,\theta,\zeta) 
\Rightarrow u_{-m,-n}(\psi) = u_{m,n}^*(\psi) \cr
\xi_\psi(\psi,\theta,\zeta) &= \xi_\psi^*(\psi,\theta,\zeta) 
\Rightarrow v_{-m,-n}(\psi) = v_{m,n}^*(\psi)
} \eqno(19) $$

$$ \eqalign{
\Xi_s(\psi) \equiv \{ u_{m,n}(\psi)\ 
	|\ m \in [m_{\rm min}, m_{\rm max}] \} \cr
\Xi_\psi(\psi) \equiv \{ v_{m,n}(\psi)\ 
	|\ m \in [m_{\rm min}, m_{\rm max}] \} \cr
} \eqno(20) $$

\vfill\eject
\centerline{\bfbig Current and Pressure Terms}
\medskip

$$ \eqalign{{\cal I}_1
\equiv& \v{J} \cdot \xi \times \v{Q} \cr
=& {\cal J} \left[(J_\zeta Q_\theta - J_\theta Q_\zeta) \xi_\psi
	+ (J_\theta \xi_\zeta - J_\zeta \xi_\theta) Q_\psi \right] \cr
=& \left\{ J_\zeta \left[{\partial \xi_s \over \partial \zeta} 
	- \left( \chi' \xi_\psi \right)' \right]
	+ J_\theta \left[ {\partial \xi_s \over \partial \theta} 
	+ \left( q \chi' \xi_\psi \right)' \right] \right\} \xi_\psi \cr
&+ \left( J_\theta \xi_\zeta - J_\zeta \xi_\theta \right) 
	\chi' \left( {\partial \over \partial \theta}
	+ q {\partial \over \partial \zeta} \right) \xi_\psi \cr
=& \xi_\psi \left( J_\theta {\partial \over \partial \theta}
	+ J_\zeta {\partial \over \partial \zeta} \right) \xi_s
	- \xi_s \left( J_\theta {\partial \over \partial \theta}
	+ J_\zeta {\partial \over \partial \zeta} \right) \xi_\psi \cr
&+ \left[ J_\theta (q \chi')' - J_\zeta \chi'' \right] \xi_\psi^2
	+ P' \left( \xi_\psi {\partial \over \partial \psi}
	+ \xi_\theta {\partial \over \partial \theta}
	+ \xi_\zeta {\partial \over \partial \zeta} \right) \xi_\psi
} \eqno(21) $$

$$ {\cal I}_2 \equiv (\xi \cdot \nabla P) (\nabla \cdot \xi)
= {\xi_\psi P' \over {\cal J}} \left[
	{\partial \over \partial \psi} \left( {\cal J} \xi_\psi \right)
	+ {\partial \over \partial \theta} \left( {\cal J} \xi_\theta \right)
	+ {\partial \over \partial \zeta} \left( {\cal J} \xi_\zeta \right)
	\right]
\eqno(22) $$

$$ \eqalign{ {\cal I}_1 + {\cal I}_2 
=& \xi_\psi \v{J} \cdot \nabla \xi_s - \xi_s \v{J} \cdot \nabla \xi_\psi
	+ \left[ J_\theta (q \chi')' - J_\zeta \chi'' \right] \xi_\psi^2 \cr
&+ {P' \over {\cal J}} \left( {\cal J} \xi_\psi^2 \right)' 
	+ {1 \over {\cal J}} {\partial \over \partial \theta} 
	\left( {\cal J} P' \xi_\psi \xi_\theta \right)
	+ {1 \over {\cal J}} {\partial \over \partial \zeta} 
	\left( {\cal J} P' \xi_\psi \xi_\zeta \right)
} \eqno(23) $$

\vfill\eject
\centerline{\bfbig Ideal MHD Stability}
\medskip

$$ \eqalign{ \delta W 
=& \int d\v{x} \left[ Q^2 + \v{J} \cdot \xi \times \v{Q}
	+ (\xi \cdot \nabla P) (\nabla \cdot \xi)
	+ \gamma P (\nabla \cdot \xi)^2 \right] \cr
=& \int d\psi d\theta d\zeta {\cal J} \biggl\{
	\Bigl[ \nabla \xi_s \times  \nabla \psi
	+ (\nabla \theta \times \nabla \zeta) 
	{\cal J} \v{B} \cdot \nabla \xi_\psi - \v{B} \xi'_\psi \cr
&\hskip1.0in - \left[ \chi'' \nabla \zeta \times \nabla \psi
	+ (q \chi')' \nabla \psi \times \nabla \theta \right] 
	\xi_\psi \Bigr]^2 \cr
& \hskip0.4in 
	+ \xi_\psi \v{J} \cdot \nabla \xi_s 
	- \xi_s \v{J} \cdot \nabla \xi_\psi
	+ \left[ J_\theta (q \chi')' - J_\zeta \chi'' \right] \xi_\psi^2
	+ {P' \over {\cal J}} \left( {\cal J} \xi_\psi^2 \right)' \cr
&\hskip0.4in
	+ {1 \over {\cal J}} {\partial \over \partial \theta} 
	\left( {\cal J} P' \xi_\psi \xi_\theta \right)
	+ {1 \over {\cal J}} {\partial \over \partial \zeta} 
	\left( {\cal J} P' \xi_\psi \xi_\zeta \right)
	+ \gamma P (\nabla \cdot \xi)^2 \biggr\} \cr
=& 4 \pi^2 \int d\psi \left[ \Xi_s^\dagger \t{A} \Xi_s 
	+ \Xi_s^\dagger (\t{B} \Xi_\psi' + \t{C} \Xi_\psi)
	+ (\Xi_\psi'^\dagger \t{B}^\dagger
	+ \Xi_\psi^\dagger \t{C}^\dagger) \Xi_s \right. \cr
&\hskip0.8in
	+ \left. \Xi_\psi'^\dagger \t{D} \Xi_\psi'
	+ \Xi_\psi'^\dagger \t{E} \Xi_\psi
	+ \Xi_\psi^\dagger \t{E}^\dagger \Xi_\psi'
	+ \Xi_\psi^\dagger \t{H} \Xi_\psi \right]
} \eqno(24) $$

$$ \eqalign{
&\t{A} \Xi_s + \t{B} \Xi_\psi' + \t{C} \Xi_\psi = 0 \cr
&\Xi_s = - \t{A}^{-1} (\t{B} \Xi_\psi' + \t{C} \Xi_\psi)
} \eqno(25) $$

$$ \eqalign{
\t{F} &\equiv \t{D} - \t{B}^\dagger \t{A}^{-1} \t{B} = \t{F}^\dagger \cr
\t{K} &\equiv \t{E} - \t{B}^\dagger \t{A}^{-1} \t{C} \ne \t{K}^\dagger \cr
\t{G} &\equiv \t{H} - \t{C}^\dagger \t{A}^{-1} \t{C} = \t{G}^\dagger
} \eqno(26) $$

$$ \delta W = 4 \pi^2 \int d\psi \left[
\Xi_\psi'^\dagger \t{F} \Xi_\psi'
+ \Xi_\psi'^\dagger \t{K} \Xi_\psi
+ \Xi_\psi^\dagger \t{K}^\dagger \Xi_\psi'
+ \Xi_\psi^\dagger \t{G} \Xi_\psi \right] 
\eqno(27) $$

$$ (\t{F} \Xi_\psi' + \t{K} \Xi_\psi)'
- (\t{K}^\dagger \Xi_\psi' + \t{G} \Xi_\psi) = 0 \eqno(28) $$

$$ \v{u} \equiv \left( \matrix{ \Xi_\psi \cr
\t{F} \Xi_\psi' + \t{K} \Xi_\psi} \right), \quad
\t{L} \equiv \left( \matrix{ 
- \t{F}^{-1} \t{K} & \t{F}^{-1} \cr
\t{G} - \t{K}^\dagger \t{F}^{-1} \t{K} & \t{K}^\dagger \t{F}^{-1}}
\right), \quad
\v{u}' = \t{L} \v{u} \eqno(29) $$

\vfill\eject
\centerline{\bfbig Coefficient Matrices}
\medskip

$$ \eqalign{
g_{11} &\equiv |\nabla \theta \times \nabla \zeta|^2 \hskip0.25in
g_{23} \equiv (\nabla \zeta \times \nabla \psi)
	\cdot (\nabla \psi \times \nabla \theta) \cr
g_{22} &\equiv |\nabla \zeta \times \nabla \psi|^2 \hskip0.25in
g_{31} \equiv (\nabla \psi \times \nabla \theta)
	\cdot (\nabla \theta \times \nabla \zeta) \cr
g_{33} &\equiv |\nabla \psi \times \nabla \theta|^2 \hskip0.25in
g_{12} \equiv (\nabla \theta \times \nabla \zeta)
	\cdot (\nabla \zeta \times \nabla \psi)
} \eqno(30) $$

$$ <{\cal F}>_{mm'} \equiv \int_0^1 d\theta {{\cal J}}
	\exp[2 \pi i (m'-m) \theta]  {\cal F}(\theta) 
\eqno(31) $$

$$ (G_{ij})_{mm'} \equiv <g_{ij}>_{mm'}
\eqno(32) $$

$$ J_{mm'} \equiv <1>_{mm'}, \quad
J'_{mm'} \equiv <{\cal J}'/{\cal J}>_{mm'}
\eqno(33) $$

$$ M_{m,m'} \equiv m \delta_{m,m'}, \quad 
Q_{m,m'} \equiv (m - n q) \delta_{m,m'} \eqno(34) $$

$$ \eqalign{
\t{A} =& (2 \pi)^2 \left[ n (n \t{G}_{22} + \t{G}_{23} \t{M}
	+\t{M} (n \t{G}_{23} + \t{G}_{33} \t{M})  \right] \cr
\t{B} =& -2 \pi i \chi' \left[ n (\t{G}_{22} + q \t{G}_{23} )
	+ \t{M} (\t{G}_{23} + q \t{G}_{33})  \right] \cr
\t{C} =& -2 \pi i \left[  \chi'' (n \t{G}_{22} + \t{M} \t{G}_{23})
	+ (q \chi')' (n \t{G}_{23} + \t{M} \t{G}_{33})  \right] \cr
	& - (2 \pi)^2 \chi' (n \t{G}_{12} + \t{M} \t{G}_{31}) \t{Q}
	+ 2 \pi i (2 \pi f' \t{Q} - n P'/\chi' \t{J}) \cr
\t{D} =& \chi'^2 \left[ (\t{G}_{22} + q \t{G}_{23})
	+ q(\t{G}_{23} + q \t{G}_{33}) \right] \cr
\t{E} =& \chi' \left[  \chi'' (\t{G}_{22} + q \t{G}_{23})
	+ (q \chi')' (\t{G}_{23} + q \t{G}_{33}) \right] \cr
	& - 2 \pi i \chi'^2 (\t{G}_{12} + q \t{G}_{31}) \t{Q}
	+ P' \t{J} \cr
\t{H} =& \chi''\left[ \chi'' \t{G}_{22} + (q \chi')' \t{G}_{23} \right]
	+ (q \chi')'\left[ \chi'' \t{G}_{23} 
	+ (q \chi')' \t{G}_{33} \right] \cr
	& + 2 \pi i \chi' \left[ \chi'' (\t{M} \t{G}_{12} - \t{G}_{12} \t{M})
	+ (q \chi')' (\t{M} \t{G}_{31} - \t{G}_{31} \t{M})  \right] \cr
	& + (2 \pi \chi')^2 \t{Q} \t{G}_{11} \t{Q}
	+ \left[ P' \left(  \t{J} \chi''/\chi' + \t{J}' \right) 
	-2 \pi f' q' \chi' \t{I} \right]
} \eqno(35) $$

$$ \eqalign{ \t{F}
\equiv& \t{D} - \t{B}^\dagger \t{A}^{-1} \t{B} \cr
=& \t{Q} (\chi' / n)^2 \left[ \t{G}_{33}
	- (n \t{G}_{23} + \t{G}_{33} \t{M}) (2 \pi)^2 \t{A}^{-1}
	(n \t{G}_{23} +  \t{M} \t{G}_{33}) \right] \t{Q}
} \eqno(36) $$

\medskip
$$ \eqalign{ \t{K}
=& \t{E} - \t{B}^\dagger \t{A}^{-1} \t{C} \cr
	=& \t{Q} (\chi'/n) \bigl\{ 2 \pi i 
	(n \t{G}_{23} + \t{G}_{33} \t{M}) \t{A}^{-1} \t{C} \cr
& - \left[  \chi'' \t{G}_{23} + (q \chi')' \t{G}_{33}
	- 2 \pi i \chi' \t{G}_{31} \t{Q} + J_\theta \t{I} \right]
\bigr\} } \eqno(37) $$

\vfill\eject
\centerline{\bfbig Change of Flux Coordinate, 1}
\medskip

$$ \eqalign{
&{\cal D} \equiv {d \psi\over d \bar{\psi}}, \quad
	{d \over d \psi} = {1 \over {\cal D}} {d \over d \bar{\psi}}, \quad
	\Xi_s = {\bar{\Xi}_s \over {\cal D}}, \quad
	\Xi_\psi = {\cal D} {\bar{\Xi}}_{\bar{\psi}} \cr
&{d \Xi_\psi \over d \psi} 
	= {1 \over {\cal D}} {d \over d \bar{\psi}}
	\left( {\cal D} {\bar{\Xi}}_{\bar{\psi}} \right)
	= {d {\bar{\Xi}}_{\bar{\psi}} \over d \bar{\psi}}
	+ \left( {1 \over {\cal D}} 
	{d {\cal D} \over d \bar{\psi}} \right)
	{\bar{\Xi}}_{\bar{\psi}} 
} \eqno(38) $$

$$ \eqalign{ \delta W 
= 4 \pi^2 \int d\psi & \left[ \Xi_s^\dagger \t{A} \Xi_s 
	+ \Xi_s^\dagger (\t{B} \Xi_\psi' + \t{C} \Xi_\psi)
	+ (\Xi_\psi'^\dagger \t{B}^\dagger
	+ \Xi_\psi^\dagger \t{C}^\dagger) \Xi_s \right. \cr
&+ \left. \Xi_\psi'^\dagger \t{D} \Xi_\psi'
	+ \Xi_\psi'^\dagger \t{E} \Xi_\psi
	+ \Xi_\psi^\dagger \t{E}^\dagger \Xi_\psi'
	+ \Xi_\psi^\dagger \t{H} \Xi_\psi \right] \cr
= 4 \pi^2 \int d\bar{\psi} & \left\{
	\bar{\Xi}_s^\dagger \t{A} \bar{\Xi}_s / {\cal D}
	+ \bar{\Xi}_s^\dagger \left[ 
	\t{B} \bar{\Xi}_{\bar{\psi}}'
	+ ( \t{B} {\cal D}' / {\cal D}
	+ \t{C} {\cal D}) \bar{\Xi}_{\bar{\psi}} \right] \right. \cr
&+ \left[ \bar{\Xi}_{\bar{\psi}}'^\dagger \t{B}^\dagger 
	+ \bar{\Xi}_{\bar{\psi}}^\dagger
	( \t{B}^\dagger {\cal D}' / {\cal D}
	+ \t{C}^\dagger {\cal D} ) \right] \bar{\Xi}_s
	+ \bar{\Xi}_{\bar{\psi}}'^\dagger \t{D} \bar{\Xi}_{\bar{\psi}}' 
	{\cal D} \cr
&+ \left[ \bar{\Xi}_{\bar{\psi}}'^\dagger 
	(\t{D} {\cal D}' + \t{E} {\cal D}^2) \bar{\Xi}_{\bar{\psi}}
	+ \bar{\Xi}_{\bar{\psi}}^\dagger 
	(\t{D}^\dagger {\cal D}' + \t{E}^\dagger {\cal D}^2) 
	\bar{\Xi}_{\bar{\psi}}'  \right] \cr
&+ \left. \bar{\Xi}_{\bar{\psi}}^\dagger 
	\left[ \t{D} {\cal D}'^2/{\cal D} 
	+ (\t{E} + \t{E}^\dagger) {\cal D}' {\cal D}
	+ \t{H} {\cal D}^3
	\right] \bar{\Xi}_{\bar{\psi}} \right\} \cr
= 4 \pi^2 \int d\bar{\psi} & \left[
	\bar{\Xi}_s^\dagger \bar{\t{A}} \bar{\Xi}_s
	+ \bar{\Xi}_s^\dagger (
	\bar{\t{B}} \bar{\Xi}_{\bar{\psi}}'
	+ \bar{\t{C}} \bar{\Xi}_{\bar{\psi}}
	+ (\bar{\Xi}_{\bar{\psi}}'^\dagger \bar{\t{B}}^\dagger
	+ \bar{\Xi}_{\bar{\psi}}^\dagger \bar{\t{C}}^\dagger
	) \bar{\Xi}_s \right. \cr
&+ \left. 
	\bar{\Xi}_{\bar{\psi}}'^\dagger \bar{\t{D}} \bar{\Xi}_{\bar{\psi}}' 
	+ \bar{\Xi}_{\bar{\psi}}'^\dagger \bar{\t{E}} \bar{\Xi}_{\bar{\psi}}
	+ \bar{\Xi}_{\bar{\psi}}^\dagger \bar{\t{E}}^\dagger 
	\bar{\Xi}_{\bar{\psi}}'
	+ \bar{\Xi}_{\bar{\psi}}^\dagger \bar{\t{H}} \bar{\Xi}_{\bar{\psi}}
	 \right]
} \eqno(39) $$

\bigskip
$$ \eqalign{
&\bar{\t{A}} = \t{A} / {\cal D}, \quad
\bar{\t{B}} = \t{B}, \quad
\bar{\t{C}} = \t{B} {\cal D}' / {\cal D} + \t{C} {\cal D} \cr
&\bar{\t{D}} = \t{D} {\cal D}, \quad
\bar{\t{E}} = \t{D} {\cal D}' + \t{E} {\cal D}^2 \cr
&\bar{\t{H}} = \t{D} {\cal D}'^2/{\cal D} 
	+ (\t{E} + \t{E}^\dagger) {\cal D}' {\cal D}
	+ \t{H} {\cal D}^3
} \eqno(40) $$

\vfill\eject
\centerline{\bfbig Change of Flux Coordinate, 2}
\medskip

$$ \eqalign{
&{\cal D} \equiv {d \psi\over d \bar{\psi}}, \quad
	{d \over d \psi} = {1 \over {\cal D}} {d \over d \bar{\psi}}, \quad
	\Xi_\psi = {\cal D} {\bar{\Xi}}_{\bar{\psi}} \cr
&{d \Xi_\psi \over d \psi} 
	= {1 \over {\cal D}} {d \over d \bar{\psi}}
	\left( {\cal D} {\bar{\Xi}}_{\bar{\psi}} \right)
	= {d {\bar{\Xi}}_{\bar{\psi}} \over d \bar{\psi}}
	+ \left( {1 \over {\cal D}} 
	{d {\cal D} \over d \bar{\psi}} \right)
	{\bar{\Xi}}_{\bar{\psi}} 
} \eqno(41) $$

$$ \eqalign{ \delta W 
= 4 \pi^2 \int d\psi & \left[
	\Xi_\psi'^\dagger \t{F} \Xi_\psi'
	+ \Xi_\psi'^\dagger \t{K} \Xi_\psi
	+ \Xi_\psi^\dagger \t{K}^\dagger \Xi_\psi'
	+ \Xi_\psi^\dagger \t{G} \Xi_\psi \right] \cr
= 4 \pi^2 \int d\bar{\psi} & \left\{
	\bar{\Xi}_{\bar{\psi}}'^\dagger \t{F} \bar{\Xi}_{\bar{\psi}}' 
	{\cal D} \right. \cr
&+ \left[ \bar{\Xi}_{\bar{\psi}}'^\dagger 
	(\t{F} {\cal D}' + \t{K} {\cal D}^2) \bar{\Xi}_{\bar{\psi}}
	+ \bar{\Xi}_{\bar{\psi}}^\dagger 
	(\t{F}^\dagger {\cal D}' + \t{K}^\dagger {\cal D}^2) 
	\bar{\Xi}_{\bar{\psi}}'  \right] \cr
&+ \left. \bar{\Xi}_{\bar{\psi}}^\dagger 
	\left[ \t{F} {\cal D}'^2/{\cal D} 
	+ (\t{K} + \t{K}^\dagger) {\cal D}' {\cal D}
	+ \t{G} {\cal D}^3
	\right] \bar{\Xi}_{\bar{\psi}} \right\} \cr
= 4 \pi^2 \int d\bar{\psi} & \left[
	\bar{\Xi}_{\bar{\psi}}'^\dagger \bar{\t{F}} \bar{\Xi}_{\bar{\psi}}' 
	+ \bar{\Xi}_{\bar{\psi}}'^\dagger \bar{\t{K}} \bar{\Xi}_{\bar{\psi}}
	+ \bar{\Xi}_{\bar{\psi}}^\dagger \bar{\t{K}}^\dagger 
	\bar{\Xi}_{\bar{\psi}}'
	+ \bar{\Xi}_{\bar{\psi}}^\dagger \bar{\t{G}} \bar{\Xi}_{\bar{\psi}}
	 \right]
} \eqno(42) $$

$$ \eqalign{
&\bar{\t{F}} = \t{F} {\cal D}, \quad
\bar{\t{K}} = \t{F} {\cal D}' + \t{K} {\cal D}^2, \quad
\bar{\t{G}} = \t{F} {\cal D}'^2/{\cal D} 
	+ (\t{K} + \t{K}^\dagger) {\cal D}' {\cal D}
	+ \t{G}\ {\cal D}^3
} \eqno(43) $$

\end
