% This is Plain TeX file metric.tex.

\magnification=\magstep2
\parskip=4pt

\font\bfbig=cmbx12
\font\ssbf=cmssbx10
\def\t#1{\hbox{\ssbf #1}}
\def\v#1{\hbox{\bf #1}}
\def\e#1{\hat {\bf e}_{#1}}

\centerline {\bfbig General 3D Coordinate Transformation}

$$ \t{J}[\v{x},\v{x}'] \equiv {\partial \over \partial \v{x}} \v{x}' 
	= {\partial x_j' \over \partial x_i}
= \left[ \matrix{
\partial x'_1 / \partial x_1
& \partial x'_2 / \partial x_1
& \partial x'_3 / \partial x_1 \cr
\partial x'_1 / \partial x_2
& \partial x'_2 / \partial x_2
& \partial x'_3 / \partial x_2 \cr
\partial x'_1 / \partial x_3
& \partial x'_2 / \partial x_3
& \partial x'_3 / \partial x_3
} \right]
\eqno(1) $$

$$ \t{J}[\v{x}',\v{x}] \equiv {\partial \over \partial \v{x}'} \v{x} 
	= {\partial x_j \over \partial x_i'}
= \left[ \matrix{
\partial x_1 / \partial x'_1
& \partial x_2 / \partial x'_1
& \partial x_3 / \partial x'_1 \cr
\partial x_1 / \partial x'_2
& \partial x_2 / \partial x'_2
& \partial x_3 / \partial x'_2 \cr
\partial x_1 / \partial x'_3
& \partial x_2 / \partial x'_3
& \partial x_3 / \partial x'_3
} \right]
\eqno(2) $$

$$ 
{\cal J} \equiv \det \t{J}[\v{r},\v{x}], \quad
{\cal J}' \equiv \det \t{J}[\v{r},\v{x}'], \quad
\t{J}[\v{x}',\v{x}] = \t{J}^{-1}[\v{x},\v{x}']
\eqno(3) $$

\medskip
$$ \eqalign{
{{\cal J} \over {\cal J}'} {\partial x_1 \over \partial x'_1}
	&= {\partial x'_2 \over \partial x_2}
	  {\partial x'_3 \over \partial x_3}
	- {\partial x'_3 \over \partial x_2}
	  {\partial x'_2 \over \partial x_3} \cr
{{\cal J} \over {\cal J}'} {\partial x_1 \over \partial x'_2}
	&= {\partial x'_3 \over \partial x_2}
	  {\partial x'_1 \over \partial x_3}
	- {\partial x'_1 \over \partial x_2}
	  {\partial x'_3 \over \partial x_3} \cr
{{\cal J} \over {\cal J}'} {\partial x_1 \over \partial x'_3}
	&= {\partial x'_1 \over \partial x_2}
	  {\partial x'_2 \over \partial x_3}
	- {\partial x'_2 \over \partial x_2}
	  {\partial x'_1 \over \partial x_3} \cr\cr
{{\cal J} \over {\cal J}'} {\partial x_2 \over \partial x'_1}
	&= {\partial x'_2 \over \partial x_3}
	  {\partial x'_3 \over \partial x_1}
	- {\partial x'_3 \over \partial x_3}
	  {\partial x'_2 \over \partial x_1} \cr
{{\cal J} \over {\cal J}'} {\partial x_2 \over \partial x'_2}
	&= {\partial x'_3 \over \partial x_3}
	  {\partial x'_1 \over \partial x_1}
	- {\partial x'_1 \over \partial x_3}
	  {\partial x'_3 \over \partial x_1} \cr
{{\cal J} \over {\cal J}'} {\partial x_2 \over \partial x'_3}
	&= {\partial x'_1 \over \partial x_3}
	  {\partial x'_2 \over \partial x_1}
	- {\partial x'_2 \over \partial x_3}
	  {\partial x'_1 \over \partial x_1} \cr\cr
{{\cal J} \over {\cal J}'} {\partial x_3 \over \partial x'_1}
	&= {\partial x'_2 \over \partial x_1}
	  {\partial x'_3 \over \partial x_2}
	- {\partial x'_3 \over \partial x_1}
	  {\partial x'_2 \over \partial x_2} \cr
{{\cal J} \over {\cal J}'} {\partial x_3 \over \partial x'_2}
	&= {\partial x'_3 \over \partial x_1}
	  {\partial x'_1 \over \partial x_2}
	- {\partial x'_1 \over \partial x_1}
	  {\partial x'_3 \over \partial x_2} \cr
{{\cal J} \over {\cal J}'} {\partial x_3 \over \partial x'_3}
	&= {\partial x'_1 \over \partial x_1}
	  {\partial x'_2 \over \partial x_2}
	- {\partial x'_2 \over \partial x_1}
	  {\partial x'_1 \over \partial x_2} \cr
} \eqno(4) $$

\vfill\eject
\centerline {\bfbig DCON Coordinate Transformation}

$$ \eqalign{
&x_1 = \psi \hskip0.25in x'_1 = r^2 \cr
&x_2 = \theta \hskip0.25in x'_2 = \eta \cr
&x_3 = \zeta \hskip0.25in x'_3 = \phi \cr
} \eqno(5) $$

$$ {\cal J}' = \pi R \eqno(6) $$

$$ {\partial r^2 \over \partial \zeta} =
{\partial \eta \over \partial \zeta} = 0, \quad
{\partial \phi \over \partial \zeta} = 2 \pi
\eqno(7) $$

\medskip
$$ \eqalign{
{{\cal J} \over {\cal J}'} {\partial \psi \over \partial r^2}
	&= {\partial \eta \over \partial \theta}
	  {\partial \phi \over \partial \zeta}
	- {\partial \phi \over \partial \theta}
	  {\partial \eta \over \partial \zeta} 
	= 2 \pi {\partial \eta \over \partial \theta} \cr
{{\cal J} \over {\cal J}'} {\partial \psi \over \partial \eta}
	&= {\partial \phi \over \partial \theta}
	  {\partial r^2 \over \partial \zeta}
	- {\partial r^2 \over \partial \theta}
	  {\partial \phi \over \partial \zeta} 
	= - 2 \pi {\partial r^2 \over \partial \theta} \cr
{{\cal J} \over {\cal J}'} {\partial \psi \over \partial \phi}
	&= {\partial r^2 \over \partial \theta}
	  {\partial \eta \over \partial \zeta}
	- {\partial \eta \over \partial \theta}
	  {\partial r^2 \over \partial \zeta} = 0\cr\cr
{{\cal J} \over {\cal J}'} {\partial \theta \over \partial r^2}
	&= {\partial \eta \over \partial \zeta}
	  {\partial \phi \over \partial \psi}
	- {\partial \phi \over \partial \zeta}
	  {\partial \eta \over \partial \psi} 
	= - 2 \pi {\partial \eta \over \partial \psi} \cr
{{\cal J} \over {\cal J}'} {\partial \theta \over \partial \eta}
	&= {\partial \phi \over \partial \zeta}
	  {\partial r^2 \over \partial \psi}
	- {\partial r^2 \over \partial \zeta}
	  {\partial \phi \over \partial \psi} 
	= 2 \pi {\partial r^2 \over \partial \psi} \cr
{{\cal J} \over {\cal J}'} {\partial \theta \over \partial \phi}
	&= {\partial r^2 \over \partial \zeta}
	  {\partial \eta \over \partial \psi}
	- {\partial \eta \over \partial \zeta}
	  {\partial r^2 \over \partial \psi} = 0 \cr\cr
{{\cal J} \over {\cal J}'} {\partial \zeta \over \partial r^2}
	&= {\partial \eta \over \partial \psi}
	  {\partial \phi \over \partial \theta}
	- {\partial \phi \over \partial \psi}
	  {\partial \eta \over \partial \theta} \cr
{{\cal J} \over {\cal J}'} {\partial \zeta \over \partial \eta}
	&= {\partial \phi \over \partial \psi}
	  {\partial r^2 \over \partial \theta}
	- {\partial r^2 \over \partial \psi}
	  {\partial \phi \over \partial \theta} \cr
{{\cal J} \over {\cal J}'} {\partial \zeta \over \partial \phi}
	&= {\partial r^2 \over \partial \psi}
	  {\partial \eta \over \partial \theta}
	- {\partial \eta \over \partial \psi}
	  {\partial r^2 \over \partial \theta} 
	= {1 \over 2 \pi} {{\cal J} \over {\cal J}'} \cr
} \eqno(8) $$

\vfill\eject
\centerline {\bfbig Contravariant Basis Vectors}

$$ \eqalign{
&\nabla r^2 = 2 r \e{1}, \quad
\nabla \eta = {\e{2} \over 2 \pi r}, \quad
\nabla \phi = {\e{3} \over R} \cr
&\e{i} \cdot \e{j} = \delta_{ij}, \quad
\e{i} \cdot \e{j} \times \e{k} = \epsilon_{ijk}
} \eqno(9) $$

$$ \eqalign{
&\v{v}_1 = \nabla \theta \times \nabla \zeta, \quad
\v{v}_2 = \nabla \zeta \times \nabla \psi, \quad
\v{v}_3 = \nabla \psi \times \nabla \theta \cr
&\v{v}_i = v_{ij} \e{j}, \quad
g_{ij} \equiv \v{v}_i \cdot \v{v}_j = v_{ik} v_{kj}
} \eqno(10) $$

$$ \eqalign{
v_{11} =& \nabla \theta \times \nabla \zeta \cdot \e{1}
	= {1 \over 2r {\cal J}'} \left(
	{\partial \theta \over \partial \eta}
	{\partial \zeta \over \partial \phi}
	- {\partial \theta \over \partial \phi}
	{\partial \zeta \over \partial \eta} \right)
	= {1 \over 2r {\cal J}} 
	{\partial r^2 \over \partial \psi} \cr 
v_{12} =& \nabla \theta \times \nabla \zeta \cdot \e{2}
	= {2\pi r \over {\cal J}'} \left(
	{\partial \theta \over \partial \phi}
	{\partial \zeta \over \partial r^2}
	- {\partial \theta \over \partial r^2}
	{\partial \zeta \over \partial \phi} \right)
	= {2\pi r \over {\cal J}} 
	{\partial \eta \over \partial \psi} \cr 
v_{13} =& \nabla \theta \times \nabla \zeta \cdot \e{3}
	= {R \over {\cal J}'} \left(
	{\partial \theta \over \partial r^2}
	{\partial \zeta \over \partial \eta}
	- {\partial \theta \over \partial \eta}
	{\partial \zeta \over \partial r^2} \right)
	= {R \over {\cal J}}
	{\partial \phi \over \partial \psi} \cr\cr
v_{21} =& \nabla \zeta \times \nabla \psi \cdot \e{1}
	= {1 \over 2r {\cal J}'} \left(
	{\partial \zeta \over \partial \eta}
	{\partial \psi \over \partial \phi}
	- {\partial \zeta \over \partial \phi}
	{\partial \psi \over \partial \eta} \right)
	= {1 \over 2r {\cal J}}
	{\partial r^2 \over \partial \theta} \cr 
v_{22} =& \nabla \zeta \times \nabla \psi \cdot \e{2}
	= {2\pi r \over {\cal J}'} \left(
	{\partial \zeta \over \partial \phi}
	{\partial \psi \over \partial r^2}
	- {\partial \zeta \over \partial r^2}
	{\partial \psi \over \partial \phi} \right)
	= {2\pi r \over {\cal J}}
	{\partial \eta \over \partial \theta} \cr 
v_{23} =& \nabla \zeta \times \nabla \psi \cdot \e{3}
	= {R \over {\cal J}'} \left(
	{\partial \zeta \over \partial r^2}
	{\partial \psi \over \partial \eta}
	- {\partial \zeta \over \partial \eta}
	{\partial \psi \over \partial r^2} \right)
	= {R \over {\cal J}}
	{\partial \phi \over \partial \theta} \cr\cr
v_{31} =& \nabla \psi \times \nabla \theta \cdot \e{1}
	= {1 \over 2r {\cal J}'} \left(
	{\partial \psi \over \partial \eta}
	{\partial \theta \over \partial \phi}
	- {\partial \psi \over \partial \phi}
	{\partial \theta \over \partial \eta} \right)
	= 0 \cr
v_{32} =& \nabla \psi \times \nabla \theta \cdot \e{2}
	= {2\pi r \over {\cal J}'} \left(
	{\partial \psi \over \partial \phi}
	{\partial \theta \over \partial r^2}
	- {\partial \psi \over \partial r^2}
	{\partial \theta \over \partial \phi} \right)
	= 0 \cr
v_{33} =& \nabla \psi \times \nabla \theta \cdot \e{3}
	= {R \over {\cal J}'} \left(
	{\partial \psi \over \partial r^2}
	{\partial \theta \over \partial \eta}
	- {\partial \psi \over \partial \eta}
	{\partial \theta \over \partial r^2} \right)
	= {R \over {\cal J}}
	{\partial \phi \over \partial \zeta} \cr\cr
} \eqno(11) $$

\vfill\eject
\centerline {\bfbig Covariant Basis Vectors}

$$ \eqalign{
&\nabla r^2 = 2 r \e{1}, \quad
\nabla \eta = {\e{2} \over 2 \pi r}, \quad
\nabla \phi = {\e{3} \over R} \cr
&\e{i} \cdot \e{j} = \delta_{ij}, \quad
\e{i} \cdot \e{j} \times \e{k} = \epsilon_{ijk}
} \eqno(12) $$

$$ \eqalign{
&\v{w}_1 = \nabla \psi, \quad
\v{w}_2 = \nabla \theta, \quad
\v{w}_3 = \nabla \zeta \cr
&\v{w}_i = w_{ij} \e{j}, \quad
{\cal J} \v{v}_i \cdot \v{w}_j = \delta_{ij}
} \eqno(13) $$

$$ \eqalign{
w_{11} =& \nabla \psi \cdot \e{1}
	= 2r {\partial \psi \over \partial r^2}
	= {4 \pi^2 rR \over {\cal J}} 
	{\partial \eta \over \partial \theta} \cr
w_{12} =& \nabla \psi \cdot \e{2}
	= {1 \over 2\pi r} {\partial \psi \over \partial \eta}
	= - {\pi R \over r {\cal J}}
	{\partial r^2 \over \partial \theta} \cr
w_{13} =& \nabla \psi \cdot \e{3}
	= {1 \over R} {\partial \psi \over \partial \phi}
	= 0 \cr\cr
w_{21} =& \nabla \theta \cdot \e{1}
	= 2r {\partial \theta \over \partial r^2}
	= - {4 \pi^2 rR \over {\cal J}}
	{\partial \eta \over \partial \psi} \cr
w_{22} =& \nabla \theta \cdot \e{2}
	= {1 \over 2\pi r} {\partial \theta \over \partial \eta}
	= {\pi R \over r {\cal J}}
	{\partial r^2 \over \partial \psi} \cr
w_{23} =& \nabla \theta \cdot \e{3}
	= {1 \over R} {\partial \theta \over \partial \phi}
	= 0 \cr\cr
w_{31} =& \nabla \zeta \cdot \e{1}
	= 2r {\partial \zeta \over \partial r^2}
	= {2 \pi rR \over {\cal J}} \left(
	{\partial \eta \over \partial \psi}
	{\partial \phi \over \partial \theta}
	- {\partial \phi \over \partial \psi}
	{\partial \eta \over \partial \theta} \right) \cr
w_{32} =& \nabla \zeta \cdot \e{2}
	= {1 \over 2\pi r} {\partial \zeta \over \partial \eta}
	= {R \over 2r {\cal J}} \left(
	{\partial \phi \over \partial \psi}
	{\partial r^2 \over \partial \theta}
	- {\partial r^2 \over \partial \psi}
	{\partial \phi \over \partial \theta} \right) \cr
w_{33} =& \nabla \zeta \cdot \e{3}
	= {1 \over R} {\partial \zeta \over \partial \phi}
	= {1 \over 2\pi R}
} \eqno(14) $$

\vfill\eject
\centerline {\bfbig Inverse Grad-Shafranov Equation}

$$ \Delta^* \chi \equiv R^2 \nabla \cdot 
	\left( {1 \over R^2} \nabla \chi \right)
	= - {4 \pi^2 \over \chi'} (ff' + R^2 P')
\eqno(15) $$

$$ {\cal J} 
	\equiv (\nabla \psi \cdot \nabla \theta \times \nabla \phi)^{-1}
\eqno(16) $$

$$ \eqalign{ {{\cal J} \over R^2} \Delta^* \chi
=& {\cal J} \nabla \cdot \left( {1 \over R^2} \nabla \chi \right) \cr
=& {\partial \over \partial \psi} \left( {\chi' {\cal J} \over R^2} 
	|\nabla \psi|^2 \right)
	+ {\partial \over \partial \theta} \left( {\chi' {\cal J} \over R^2} 
	\nabla \psi \cdot \nabla \theta \right) \cr
=& {\partial \over \partial \psi} \left\{ {\chi' {\cal J} \over R^2}
	\left[ 4 r^2 \left({\partial \psi \over \partial r^2} \right)^2
	+ {1 \over 4 \pi^2 r^2} \left( 
	{\partial \psi \over \partial \eta} \right)^2 \right] \right\} \cr
&+ {\partial \over \partial \theta} \left\{ {\chi' {\cal J} \over R^2}
	\left[ 4 r^2 
	{\partial \psi \over \partial r^2}
	{\partial \theta \over \partial r^2}
	+ {1 \over 4 \pi^2 r^2} 
	{\partial \psi \over \partial \eta}
	{\partial \theta \over \partial \eta}
	\right] \right\} \cr
=& {\partial \over \partial \psi} \left\{ 
	{4 \pi^4 \chi' \over {\cal J}}
	\left[ 4 r^2 
	\left({\partial \eta \over \partial \theta} \right)^2
	+ {1 \over 4 \pi^2 r^2} 
	\left({\partial r^2 \over \partial \theta} \right)^2 
	\right] \right\} \cr
&- {\partial \over \partial \theta} \left\{ 
	{4 \pi^4 \chi' \over {\cal J}}
	\left[ 4 r^2 
	{\partial \eta \over \partial \theta}
	{\partial \eta \over \partial \psi}
	+ {1 \over 4 \pi^2 r^2} 
	{\partial r^2 \over \partial \theta}
	{\partial r^2 \over \partial \psi}
	\right] \right\} \cr
} \eqno(17) $$

$$ \eqalign{ 
& {\partial \over \partial \psi} \left\{ 
	{\chi' \over {\cal J}}
	\left[ 4 r^2 
	\left({\partial \eta \over \partial \theta} \right)^2
	+ {1 \over 4 \pi^2 r^2} 
	\left({\partial r^2 \over \partial \theta} \right)^2 
	\right] \right\} \cr
& \quad - {\partial \over \partial \theta} \left\{ 
	{\chi' \over {\cal J}}
	\left[ 4 r^2 
	{\partial \eta \over \partial \theta}
	{\partial \eta \over \partial \psi}
	+ {1 \over 4 \pi^2 r^2} 
	{\partial r^2 \over \partial \theta}
	{\partial r^2 \over \partial \psi}
	\right] \right\} \cr
&\quad = - {1 \over \pi^2 R^2} {{\cal J} \over \chi'} (ff' + R^2 P')
} \eqno(18) $$

\end
